started trying to define monad operations for the trace monad using logical relations...

theories/TraceMonad.v
@@ -1,9 +1,93 @@
 Require Export Coq.Relations.Relations.
 Require Export Coq.Classes.RelationClasses.
+Require Export Coq.Classes.Morphisms.
+Require Export Coq.Setoids.Setoid.
 
 
 (***
- *** Computation Trees
+ *** Logical Relations
+ ***)
+
+Class LR A : Type :=
+  { lr_leq : relation A; lr_PreOrder :> PreOrder lr_leq }.
+
+Instance LR_Reflexive A `{LR A} : Reflexive lr_leq.
+Proof. typeclasses eauto. Qed.
+
+Instance LR_Transitive A `{LR A} : Transitive lr_leq.
+Proof. typeclasses eauto. Qed.
+
+(* The equivalence relation for a logical relation *)
+Definition lr_equiv {A} `{LR A} : relation A :=
+  fun x y => lr_leq x y /\ lr_leq y x.
+
+Instance lr_equiv_Equivalence A `{LR A} : Equivalence lr_equiv.
+Proof.
+  constructor; intro; intros.
+  { split; reflexivity. }
+  { destruct H0; split; assumption. }
+  { destruct H0; destruct H1; split; transitivity y; assumption. }
+Qed.
+
+Notation "x <lr= y" :=
+  (lr_leq x y) (no associativity, at level 70).
+Notation "x =lr= y" :=
+  (lr_equiv x y) (no associativity, at level 70).
+
+(* FIXME: figure out what versions of this we need for rewriting! *)
+Instance Proper_lr_leq_lr_leq A `{LR A}
+  : Proper (lr_leq --> lr_leq ==> Basics.impl) (@lr_leq A _).
+Proof.
+  intros a1 a2 Ra b1 b2 Rb Rab.
+  transitivity a1; [ assumption | ]. transitivity b1; assumption.
+Qed.
+
+Instance Subrelation_lr_equiv_lr_leq A `{LR A} :
+  subrelation (@lr_equiv A _) lr_leq.
+Proof.
+  intros a1 a2 Ra; destruct Ra; assumption.
+Qed.
+
+Instance Proper_lr_equiv_lr_leq A `{LR A} :
+  Proper (lr_equiv ==> lr_equiv ==> iff) (@lr_leq A _).
+Proof.
+  intros x1 x2 Rx y1 y2 Ry; destruct Rx; destruct Ry; split; intro Rxy.
+  transitivity x1; [ assumption | ]; transitivity y1; assumption.
+  transitivity x2; [ assumption | ]; transitivity y2; assumption.
+Qed.
+
+Instance Proper_lr_equiv A `{LR A} :
+  Proper (lr_equiv ==> lr_equiv ==> iff) (@lr_equiv A _).
+Proof.
+  intros x1 x2 Rx y1 y2 Ry. rewrite Rx. rewrite Ry. reflexivity.
+Qed.
+
+Instance Proper_lr_equiv_partial A `{LR A} a :
+  Proper (lr_equiv ==> Basics.flip Basics.impl) (@lr_equiv A _ a).
+Proof.
+  intros x1 x2 Rx. rewrite Rx. reflexivity.
+Qed.
+
+
+Instance LR_arrow {A B} `{LR B} : LR (A -> B) :=
+  { lr_leq := fun f g => forall a, f a <lr= g a }.
+Proof.
+  constructor.
+  - intros f a. reflexivity.
+  - intros f g h Rfg Rgh a. transitivity (g a); [ apply Rfg | apply Rgh ].
+Defined.
+
+Instance LR_Prop : LR Prop :=
+  { lr_leq := Basics.impl }.
+Proof.
+  constructor.
+  - intros P H; assumption.
+  - intros P1 P2 P3 impl12 impl23 pf; apply impl23; apply impl12; assumption.
+Defined.
+
+
+(***
+ *** Finite Computation Trees
  ***)
 
 Inductive FinCompTree St A : Type :=
@@ -29,14 +113,25 @@ Instance PreOrder_extendsFCT {St A} : PreOrder (@extendsFCT St A).
 Proof.
   constructor.
   - intros tree; induction tree; simpl; auto.
-  - intros tree1; induction tree1; intros tree2 tree3;
-      destruct tree2; destruct tree3; simpl; intros;
+  - intros tree1; induction tree1 as [ | | s a IH ];
+      intros tree2 tree3;
+      destruct tree2; destruct tree3; simpl; intros R12 R23;
         try auto; try contradiction.
-    + destruct H; destruct H0; rewrite H; rewrite H0; rewrite H1; rewrite H2.
-      split; reflexivity.
-    + destruct H0; destruct H1. rewrite H0; rewrite H1; split; [ reflexivity | ].
-      intro. apply (H _ _ _ (H2 _) (H3 _)).
+    + destruct R12 as [ Rs12 Ra12 ]; destruct R23 as [ Rs23 Ra23 ].
+      split; [ rewrite Rs12; rewrite Rs23 | rewrite Ra12; rewrite Ra23 ];
+        reflexivity.
+    + destruct R12 as [ Rs12 Ra12 ]; destruct R23 as [ Rs23 Ra23 ].
+      split; [ rewrite Rs12; rewrite Rs23; reflexivity | ].
+      intro. apply (IH _ _ _ (Ra12 _) (Ra23 _)).
 Qed.
+
+Instance LR_FinCompTree {St A} : LR (FinCompTree St A) :=
+  { lr_leq := extendsFCT; lr_PreOrder := _ }.
+
+
+(***
+ *** Computation Trees
+ ***)
 
 (* A "computation tree" is a prefix-closed set of finite trees *)
 Record CompTree St A : Type :=
@@ -47,17 +142,93 @@ Record CompTree St A : Type :=
 Arguments ctIn {St A} _.
 Arguments ctClosed {St A} _.
 
-Definition extendsFT {St A} : relation (CompTree St A) :=
-  fun tree1 tree2 =>
-    forall fct, ctIn tree1 fct -> ctIn tree2 fct.
-
-Instance PreOrder_extendsFT {St A} : PreOrder (@extendsFT St A).
+Instance LR_CompTree St A : LR (CompTree St A) :=
+  { lr_leq := fun tree1 tree2 => lr_leq (ctIn tree1) (ctIn tree2) }.
 Proof.
   constructor.
-  - intros tree fct H; assumption.
-  - intros tree1 tree2 tree3 R12 R23 fct fct_in.
-    apply R23. apply R12. assumption.
+  - intro. reflexivity.
+  - intros tree1 tree2 tree3; transitivity (ctIn tree2); assumption.
 Qed.
+
+
+Program Definition downCloseTree {St A} tree : CompTree St A :=
+  {|
+    ctIn := fun tree' => lr_leq tree' tree;
+  |}.
+Next Obligation.
+  etransitivity; eassumption.
+Defined.
+
+Instance Proper_downCloseTree St A :
+  Proper (lr_leq ==> lr_leq) (@downCloseTree St A).
+Proof.
+  admit. (* FIXME HERE *)
+Admitted.
+
+
+(***
+ *** Stateful Monads
+ ***)
+
+Class MonadStateOps M St : Type :=
+  {
+    returnM : forall {A}, A -> M A;
+    bindM : forall {A B}, M A -> (A -> M B) -> M B;
+    getM : M St;
+    putM : St -> M unit;
+  }.
+
+Class MonadState M St `{MonadStateOps M St} : Type :=
+  {
+    Monad_LR {A} :> LR (M A);
+
+    Proper_bindM {A B} :
+      Proper (lr_leq ==> lr_leq ==> lr_leq) (bindM (A:=A) (B:=B));
+
+    monad_return_bind {A B} a (f : A -> M B) :
+      bindM (returnM a) f =lr= f a;
+    monad_bind_return {A} (m : M A) :
+      bindM m returnM =lr= m;
+    monad_assoc {A B C} m (f: A -> M B) (g: B -> M C) :
+      bindM (bindM m f) g =lr= bindM m (fun x => bindM (f x) g);
+
+    (* FIXME HERE: write the monad laws! *)
+  }.
+
+
+(***
+ *** The Finite Trace Monad
+ ***)
+
+Definition FinTraceMonad St A := St -> FinCompTree St A.
+
+Fixpoint bindFinTree {St A B} (fct: FinCompTree St A)
+         (f : A -> FinTraceMonad St B) : FinCompTree St B :=
+  match fct with
+  | TreeStuck => TreeStuck
+  | TreeLeaf s a => f a s
+  | TreeNode s step =>
+    TreeNode s (fun s' => bindFinTree (step s') f)
+  end.
+
+Instance Proper_bindFinTree St A B :
+  Proper (lr_leq ==> lr_leq ==> lr_leq) (@bindFinTree St A B).
+Proof.
+  admit. (* FIXME HERE *)
+Admitted.
+
+Instance MonadStateOps_FinTraceMonad St : MonadStateOps (FinTraceMonad St) St :=
+  {|
+    returnM := fun A a s => TreeLeaf s a;
+    bindM := fun A B m f s => bindFinTree (m s) f;
+    getM := fun s => TreeLeaf s s;
+    putM := fun s _ => TreeLeaf s tt
+  |}.
+
+Instance MonadState_FinTraceMonad St : MonadState (FinTraceMonad St) St.
+Proof.
+  admit. (* FIXME HERE *)
+Admitted.
 
 
 (***
@@ -66,15 +237,30 @@ Qed.
 
 Definition TraceMonad St A := St -> CompTree St A.
 
-Definition FinTraceMonad St A := St -> FinCompTree St A.
+Definition downCloseM {St A} (m: FinTraceMonad St A) : TraceMonad St A :=
+  fun s => downCloseTree (m s).
 
-Definition extendsFTM {St A} : relation (FinTraceMonad St A) :=
-  fun m1 m2 => forall s, extendsFCT (m1 s) (m2 s).
 
-Definition approxTM {St A} (m: TraceMonad St A) (ftm: FinTraceMonad St A) : Prop :=
+FIXME HERE NOW: write bindTree!
+
+Program Definition bindTree {St A B} (tree: CompTree St A)
+        (f: A -> TraceMonad St B) : CompTree St B :=
+  {| ctIn := fun ftreeB =>
+               exists 
+
+Instance MonadStateOps_TraceMonad St : MonadStateOps (TraceMonad St) St :=
+  {|
+    returnM := fun A a => downCloseM (returnM a);
+    bindM :=
+      fun A B m f =>
+        
+
+
+Definition approxTM {St A} `{LR A}
+           (m: TraceMonad St A) (ftm: FinTraceMonad St A) : Prop :=
   forall s, ctIn (m s) (ftm s).
 
-Definition stepsTo1 {St A} : relation (St * TraceMonad St A) :=
+Definition stepsTo1 {St A} `{LR A} : relation (St * TraceMonad St A) :=
   fun stm1 stm2 =>
     forall ftm,
       approxTM (snd stm2) ftm
